minuska/theories/syntax_properties.v
@@ -3,151 +3,212 @@ From Minuska Require Import
     spec_syntax
 .
 
- Section vars_of.
+Definition vars_of_AP
+    {Σ : Signature}
+    (ap : AtomicProposition)
+    : gset variable :=
+match ap with
+| ap1 _ x => {[x]}
+| ap2 _ x y => {[x;y]}
+end.
 
-    Definition vars_of_AP
-        {Σ : Signature}
-        (ap : AtomicProposition)
-        : gset variable :=
-    match ap with
-    | ap1 _ x => {[x]}
-    | ap2 _ x y => {[x;y]}
-    end.
+Fixpoint vars_of_Constraint
+    { Σ : Signature }
+    (c : Constraint)
+    : gset variable :=
+match c with
+| c_True => ∅
+| c_atomic ap => vars_of_AP ap
+| c_and c1 c2 => vars_of_Constraint c1 ∪ vars_of_Constraint c2
+| c_not c' => vars_of_Constraint c'
+end.
 
-    Fixpoint vars_of_Constraint
-        { Σ : Signature }
-        (c : Constraint)
-        : gset variable :=
-    match c with
-    | c_True => ∅
-    | c_atomic ap => vars_of_AP ap
-    | c_and c1 c2 => vars_of_Constraint c1 ∪ vars_of_Constraint c2
-    | c_not c' => vars_of_Constraint c'
-    end.
+Fixpoint vars_of_aosb
+    {Σ : Signature}
+    (o : AppliedOperator' symbol BuiltinOrVar)
+    : gset variable :=
+match o with
+| ao_operator _ => ∅
+| ao_app_operand o' (bov_builtin _) => vars_of_aosb o'
+| ao_app_operand o' (bov_variable x) => {[x]} ∪ vars_of_aosb o'
+| ao_app_ao o1 o2 => vars_of_aosb o1 ∪ vars_of_aosb o2
+end.
 
-    Fixpoint vars_of_aosb
-        {Σ : Signature}
-        (o : AppliedOperator' symbol BuiltinOrVar)
-        : gset variable :=
-    match o with
-    | ao_operator _ => ∅
-    | ao_app_operand o' (bov_builtin _) => vars_of_aosb o'
-    | ao_app_operand o' (bov_variable x) => {[x]} ∪ vars_of_aosb o'
-    | ao_app_ao o1 o2 => vars_of_aosb o1 ∪ vars_of_aosb o2
-    end.
+Definition vars_of_OpenTerm
+    {Σ : Signature}
+    (φ : OpenTerm)
+    : gset variable :=
+match φ with
+| aoo_app _ _ o => vars_of_aosb o
+| aoo_operand _ _ (bov_variable x) => {[x]}
+| aoo_operand _ _ (bov_builtin _) => ∅
+end.
 
-    Definition vars_of_OpenTerm
-        {Σ : Signature}
-        (φ : OpenTerm)
-        : gset variable :=
-    match φ with
-    | aoo_app _ _ o => vars_of_aosb o
-    | aoo_operand _ _ (bov_variable x) => {[x]}
-    | aoo_operand _ _ (bov_builtin _) => ∅
-    end.
-    
-    Definition vars_of_SideCondition
-        {Σ : Signature}
-        (c : SideCondition)
-        : gset variable :=
-    match c with
-    | sc_constraint c' => vars_of_Constraint c'
-    | sc_match x φ => {[x]} ∪ vars_of_OpenTerm φ
-    end.
+Definition vars_of_SideCondition
+    {Σ : Signature}
+    (c : SideCondition)
+    : gset variable :=
+match c with
+| sc_constraint c' => vars_of_Constraint c'
+| sc_match x φ => {[x]} ∪ vars_of_OpenTerm φ
+end.
 
-    Fixpoint vars_of_OpenTermWSC
-        {Σ : Signature}
-        (φc : OpenTermWSC)
-        : gset variable :=
-    match φc with
-    | wsc_base φ => vars_of_OpenTerm φ
-    | wsc_sc φ c
-        => vars_of_OpenTermWSC φ ∪ vars_of_SideCondition c
-    end.
+Fixpoint vars_of_OpenTermWSC
+    {Σ : Signature}
+    (φc : OpenTermWSC)
+    : gset variable :=
+match φc with
+| wsc_base φ => vars_of_OpenTerm φ
+| wsc_sc φ c
+    => vars_of_OpenTermWSC φ ∪ vars_of_SideCondition c
+end.
 
-    Fixpoint vars_of_AppliedOperator'_symbol_OpenTermWSC
-        {Σ : Signature}
-        (φ : AppliedOperator' symbol OpenTermWSC)
-        : gset variable :=
-    match φ with
-    | ao_operator o => ∅
-    | ao_app_operand x y
-        => vars_of_AppliedOperator'_symbol_OpenTermWSC x ∪ vars_of_OpenTermWSC y
-    | ao_app_ao x y
-        => vars_of_AppliedOperator'_symbol_OpenTermWSC x ∪ vars_of_AppliedOperator'_symbol_OpenTermWSC y
-    end.
+Fixpoint vars_of_AppliedOperator'_symbol_OpenTermWSC
+    {Σ : Signature}
+    (φ : AppliedOperator' symbol OpenTermWSC)
+    : gset variable :=
+match φ with
+| ao_operator o => ∅
+| ao_app_operand x y
+    => vars_of_AppliedOperator'_symbol_OpenTermWSC x ∪ vars_of_OpenTermWSC y
+| ao_app_ao x y
+    => vars_of_AppliedOperator'_symbol_OpenTermWSC x ∪ vars_of_AppliedOperator'_symbol_OpenTermWSC y
+end.
 
-    Definition vars_of_LhsPattern
-        {Σ : Signature}
-        (φ : LhsPattern)
-        : gset variable :=
-    match φ with
-    | aoo_app _ _ aop => vars_of_AppliedOperator'_symbol_OpenTermWSC aop
-    | aoo_operand _ _ otwsc => vars_of_OpenTermWSC otwsc
-    end.
+Definition vars_of_LhsPattern
+    {Σ : Signature}
+    (φ : LhsPattern)
+    : gset variable :=
+match φ with
+| aoo_app _ _ aop => vars_of_AppliedOperator'_symbol_OpenTermWSC aop
+| aoo_operand _ _ otwsc => vars_of_OpenTermWSC otwsc
+end.
 
-    Fixpoint vars_of_Expression
-        {Σ : Signature}
-        (t : Expression)
-        : gset variable :=
-    match t with
-    | ft_element _ => ∅
-    | ft_variable x => {[x]}
-    | ft_unary _ t' => vars_of_Expression t'
-    | ft_binary _ t1 t2 => vars_of_Expression t1 ∪ vars_of_Expression t2
-    end.
+Fixpoint vars_of_Expression
+    {Σ : Signature}
+    (t : Expression)
+    : gset variable :=
+match t with
+| ft_element _ => ∅
+| ft_variable x => {[x]}
+| ft_unary _ t' => vars_of_Expression t'
+| ft_binary _ t1 t2 => vars_of_Expression t1 ∪ vars_of_Expression t2
+end.
 
-    Fixpoint vars_of_AppliedOperator_sym_fterm
-        {Σ : Signature}
-        (op : AppliedOperator' symbol Expression)
-        : gset variable :=
-    match op with
-    | ao_operator _ => ∅
-    | ao_app_operand aps' o =>
-        vars_of_AppliedOperator_sym_fterm aps' ∪ vars_of_Expression o
-    | ao_app_ao aps1 aps2 =>
-        vars_of_AppliedOperator_sym_fterm aps1 ∪ vars_of_AppliedOperator_sym_fterm aps2
-    end.
+Fixpoint vars_of_AppliedOperator_sym_fterm
+    {Σ : Signature}
+    (op : AppliedOperator' symbol Expression)
+    : gset variable :=
+match op with
+| ao_operator _ => ∅
+| ao_app_operand aps' o =>
+    vars_of_AppliedOperator_sym_fterm aps' ∪ vars_of_Expression o
+| ao_app_ao aps1 aps2 =>
+    vars_of_AppliedOperator_sym_fterm aps1 ∪ vars_of_AppliedOperator_sym_fterm aps2
+end.
 
-    Fixpoint vars_of_AppliedOperator'_symbol_Expression
-        {Σ : Signature}
-        (φ : AppliedOperator' symbol Expression)
-        : gset variable :=
-    match φ with
-    | ao_operator _ => ∅
-    | ao_app_operand  φ' t
-        => vars_of_AppliedOperator'_symbol_Expression φ' ∪ vars_of_Expression t
-    | ao_app_ao φ1 φ2
-        => vars_of_AppliedOperator'_symbol_Expression φ1 ∪ vars_of_AppliedOperator'_symbol_Expression φ2
-    end.
+Fixpoint vars_of_AppliedOperator'_symbol_Expression
+    {Σ : Signature}
+    (φ : AppliedOperator' symbol Expression)
+    : gset variable :=
+match φ with
+| ao_operator _ => ∅
+| ao_app_operand  φ' t
+    => vars_of_AppliedOperator'_symbol_Expression φ' ∪ vars_of_Expression t
+| ao_app_ao φ1 φ2
+    => vars_of_AppliedOperator'_symbol_Expression φ1 ∪ vars_of_AppliedOperator'_symbol_Expression φ2
+end.
 
-    Definition vars_of_RhsPattern
-        {Σ : Signature}
-        (φ : RhsPattern)
-        : gset variable :=
-    match φ with
-    | aoo_app _ _ aop => vars_of_AppliedOperator'_symbol_Expression aop
-    | aoo_operand _ _ exp => vars_of_Expression exp
-    end.
+Definition vars_of_RhsPattern
+    {Σ : Signature}
+    (φ : RhsPattern)
+    : gset variable :=
+match φ with
+| aoo_app _ _ aop => vars_of_AppliedOperator'_symbol_Expression aop
+| aoo_operand _ _ exp => vars_of_Expression exp
+end.
 
-    Fixpoint var_of_WithASideCondition_variable
-        {Σ : Signature}
-        (x : WithASideCondition variable)
-        : variable :=
-    match x with
-    | wsc_base x' => x'
-    | wsc_sc x' sc => var_of_WithASideCondition_variable x'
-    end.
+Fixpoint var_of_WithASideCondition_variable
+    {Σ : Signature}
+    (x : WithASideCondition variable)
+    : variable :=
+match x with
+| wsc_base x' => x'
+| wsc_sc x' sc => var_of_WithASideCondition_variable x'
+end.
 
-    Definition vars_of_LocalRewrite
-        {Σ : Signature}
-        (lr : LeftRight)
-        (r : LocalRewrite)
-        : gset variable :=
-    match lr,r with
-    | LR_Left, Build_LocalRewrite _ φ1 φ2 => vars_of_LhsPattern φ1
-    | LR_Right, Build_LocalRewrite _ φ1 φ2 => vars_of_RhsPattern φ2
-    end.
+Definition vars_of_LocalRewrite
+    {Σ : Signature}
+    (lr : LeftRight)
+    (r : LocalRewrite)
+    : gset variable :=
+match lr,r with
+| LR_Left, Build_LocalRewrite _ φ1 φ2 => vars_of_LhsPattern φ1
+| LR_Right, Build_LocalRewrite _ φ1 φ2 => vars_of_RhsPattern φ2
+end.
 
 
-End vars_of.
+Fixpoint AppliedOperator'_fmap
+    {A B C : Type}
+    (f : B -> C)
+    (ao : AppliedOperator' A B)
+    : AppliedOperator' A C
+:=
+match ao with
+| ao_operator o => ao_operator o
+| ao_app_operand ao' x => ao_app_operand (AppliedOperator'_fmap f ao') (f x)
+| ao_app_ao ao1 ao2 => ao_app_ao (AppliedOperator'_fmap f ao1) (AppliedOperator'_fmap f ao2)
+end.
+
+Definition AppliedOperatorOr'_fmap
+    {A B C : Type}
+    (f : B -> C)
+    (aoo : AppliedOperatorOr' A B)
+    : AppliedOperatorOr' A C
+:=
+match aoo with
+| aoo_app _ _ ao => aoo_app _ _ (AppliedOperator'_fmap f ao)
+| aoo_operand _ _ o => aoo_operand _ _ (f o)
+end.
+
+
+#[global]
+Instance AppliedOperatorOr'_A_B_fmap (A : Type)
+    : FMap (AppliedOperatorOr' A)
+    := @AppliedOperatorOr'_fmap A
+.
+
+Fixpoint AppliedOperator'_collapse_option
+    {A B : Type}
+    (ao : AppliedOperator' A (option B))
+    : option (AppliedOperator' A B)
+:=
+match ao with
+| ao_operator o =>
+    Some (ao_operator o)
+
+| ao_app_operand ao' x =>
+    ao'' ← AppliedOperator'_collapse_option ao';
+    x'' ← x;
+    Some (ao_app_operand ao'' x'')
+
+| ao_app_ao ao1 ao2 =>
+    ao1'' ← AppliedOperator'_collapse_option ao1;
+    ao2'' ← AppliedOperator'_collapse_option ao2;
+    Some (ao_app_ao ao1'' ao2'')
+end.
+
+
+Definition AppliedOperatorOr'_collapse_option
+    {A B : Type}
+    (aoo : AppliedOperatorOr' A (option B))
+    : option (AppliedOperatorOr' A B)
+:=
+match aoo with
+| aoo_app _ _ ao =>
+    tmp ← AppliedOperator'_collapse_option ao;
+    Some (aoo_app _ _ tmp)
+| aoo_operand _ _ op =>
+    tmp ← op;
+    Some (aoo_operand _ _ tmp)
+end.
