minuska/theories/flattened.v
@@ -1,0 +1,43 @@
+From Minuska Require Import
+    prelude
+    tactics
+    spec_syntax
+    spec_semantics
+.
+
+
+
+Definition valuation_satisfies_scs
+    {Σ : Signature}
+    (ρ : Valuation)
+    (scs : list SideCondition)
+    : Prop
+:= Forall (valuation_satisfies_sc ρ) scs
+.
+
+Record FlattenedRewritingRule {Σ : Signature} := {
+    fr_from : OpenTerm ;
+    fr_to : RhsPattern ;
+    fr_scs : list SideCondition ;
+}.
+
+Definition flattened_rewrites_in_valuation_to
+    {Σ : Signature}
+    (ρ : Valuation)
+    (r : FlattenedRewritingRule)
+    (from to : GroundTerm)
+    : Prop
+:= in_val_GroundTerm_satisfies_OpenTerm
+    ρ from (fr_from r)
+/\ GroundTerm_satisfies_RhsPattern
+    ρ to (fr_to r)
+/\ valuation_satisfies_scs ρ (fr_scs r)
+.
+
+Definition flattened_rewrites_to
+    {Σ : Signature}
+    (r : FlattenedRewritingRule)
+    (from to : GroundTerm)
+    : Prop
+:= exists ρ, flattened_rewrites_in_valuation_to ρ r from to
+.
